lithium/type.v
@@ -248,6 +248,8 @@ Record type `{!typeG Σ} {cs : compspecs} := {
   ty_own : own_state → address → iProp Σ;
   (** [ty_own v ty], also [v ◁ᵥ ty], states that the value [v] has type [ty]. *)
   ty_own_val : val → iProp Σ;
+  (** [ty_own v ty], also [v ◁ᵥ ty], states that the value [v] has type [ty]. *)
+  ty_own_val_affine v : Affine (ty_own_val v);
   (** [ty_share] states that full ownership can always be turned into shared ownership. *)
   ty_share l E : ↑shrN ⊆ E → ty_own Own l ={E}=∗ ty_own Shr l;
   (** [ty_shr_pers] states that shared ownership is persistent. *)
@@ -282,6 +284,7 @@ Record type `{!typeG Σ} {cs : compspecs} := {
 Arguments ty_own : simpl never.
 Arguments ty_has_op_type {_ _ _} _.
 Arguments ty_own_val {_ _ _} _ : simpl never.
+Global Existing Instance ty_own_val_affine.
 Global Existing Instance ty_shr_pers.
 
 (*Section memcast.
@@ -435,7 +438,7 @@ Section true.
   Program Definition tytrue : type := {|
     ty_own _ _ := True%I;
     ty_has_op_type _ _ := False%type;
-    ty_own_val _ := True%I;
+    ty_own_val _ := emp;
   |}.
   Solve Obligations with try done.
   Next Obligation. iIntros (???) "?". done. Qed.
